PrintAxioms.lean
@@ -976,7 +976,7 @@ import Compiler.Proofs.YulGeneration.Equivalence
 #print axioms Compiler.Proofs.IRGeneration.FunctionBody.runtimeStateMatchesIR_setVar_bindValue
 #print axioms Compiler.Proofs.IRGeneration.FunctionBody.runtimeStateMatchesIR_setVar_irrelevant
 #print axioms Compiler.Proofs.IRGeneration.FunctionBody.compileStmt_core_ok
-#print axioms Compiler.Proofs.IRGeneration.FunctionBody.runtimeStateMatchesIR_setMemory
+#print axioms Compiler.Proofs.IRGeneration.FunctionBody.runtimeStateMatchesIR_setBothMemory
 #print axioms Compiler.Proofs.IRGeneration.FunctionBody.runtimeStateMatchesIR_setTransientStorage
 #print axioms Compiler.Proofs.IRGeneration.FunctionBody.bindingsExactlyMatchIRVars_setMemory
 #print axioms Compiler.Proofs.IRGeneration.FunctionBody.bindingsExactlyMatchIRVarsOnScope_setMemory
